src/lib/sparse/Kuiper.Sparse.PtsTo.fst
@@ -1,0 +1,480 @@
+module Kuiper.Sparse.PtsTo
+
+#lang-pulse
+
+open Kuiper
+open FStar.Tactics.V2 { exact }
+open Kuiper.Array.Vectorized
+open Kuiper.Sparse.Common
+
+
+(* Live *)
+
+let slice_live
+  (#et : Type0)
+  (#l : nat)
+  (a : gpu_array et l)
+  (#[FStar.Tactics.exact (`1.0R)] f : perm)
+  (i j : nat)
+  : slprop
+  = exists* s. gpu_pts_to_slice a #f i j s
+
+let array_live_cell
+  (#et : Type0)
+  (#l : nat)
+  (a :gpu_array et l)
+  (#[FStar.Tactics.exact (`1.0R)] f : perm)
+  (i : natlt l)
+  : slprop
+  = exists* v. gpu_pts_to_cell a #f i v
+
+module Array2 = Kuiper.Array2
+
+let matrix_live_cell
+  (#et : Type0)
+  (#rows #cols : nat)
+  (#lm : Array2.layout rows cols)
+  (gm : Array2.t et lm)
+  (i : natlt rows)
+  (j : natlt cols)
+  : slprop
+  = exists* v. Array2.pts_to_cell gm (i, j) v
+
+
+(* Vector *)
+
+unfold
+let gpu_pts_to_vec
+  (#a:Type u#0) {| sized a, has_vec_cpy a |}
+  (#sz:nat)
+  ([@@@mkey] x:gpu_array a sz)
+  (#[exact (`1.0R)] f : perm)
+  ([@@@mkey] i : nat)
+  (v : seq a)
+: slprop
+= 
+  gpu_pts_to_slice x #f i (i + chunk a) v
+
+unfold
+let gpu_pts_to_vec'
+  (#a:Type) {| sized a, has_vec_cpy a |}
+  (#sz:nat)
+  ([@@@mkey] x:gpu_array a sz)
+  (#[exact (`1.0R)] f : perm)
+  ([@@@mkey] i : nat)
+  (v : seq a)
+  (k : natle (len v - chunk a))
+: slprop
+= gpu_pts_to_vec x #f i (Seq.slice v k (k + chunk a))
+
+let gpu_live_vec
+  (#a:Type) {| sized a, has_vec_cpy a |}
+  (#l : nat)
+  (x :gpu_array a l)
+  (#[exact (`1.0R)] f : perm)
+  (i : nat)
+: slprop
+= exists* v. gpu_pts_to_vec x #f i v
+
+
+
+(* Thread sharing *)
+
+let thread_slice_pts_to
+  (#et : Type0)
+  (#n : nat)
+  (a : gpu_array et n)
+  (i j : natle n { i <= j })
+  (#m : nat)
+  (s : lseq et m)
+  (k : natle (m - (j - i)))
+  (nthr : nat) (tid : natlt nthr)
+: slprop
+=
+  forall+ (x : natlt ((j - i - tid) `divup` nthr)).
+    gpu_pts_to_cell a (i + x * nthr + tid) (s @! k + x * nthr + tid)
+
+let thread_slice_pts_to_value
+  (#et : Type0)
+  (#n : nat)
+  (a : gpu_array et n)
+  (i j : natle n { i <= j })
+  (v : et)
+  (nthr : nat) (tid : natlt nthr)
+: slprop
+=
+  forall+ (x : natlt ((j - i - tid) `divup` nthr)).
+    gpu_pts_to_cell a (i + x * nthr + tid) v
+
+let thread_slice_live
+  (#et : Type0)
+  (#n : nat)
+  (a : gpu_array et n)
+  (i j : natle n {i <= j})
+  (nthr : nat) (tid : natlt nthr)
+: slprop
+=
+  forall+ (k : natlt ((j - i - tid) `divup` nthr)).
+    array_live_cell a (i + k * nthr + tid)
+
+
+(* Vector thread sharing *)
+
+let thread_pts_to_chunks
+  (#et : Type0) {| sized et, has_vec_cpy et |}
+  (#n : nat)
+  ([@@@mkey] x : gpu_array et n)
+  (#m : nat)
+  (s : lseq et m)
+  (i : nat)
+  (nthr : nat)
+  (tid : natlt nthr)
+: Pure slprop
+  (requires (nthr * chunk et) /? n /\ i + n <= m)
+  (ensures fun _ -> true)
+=
+  forall+ (k : natlt (n / (nthr * chunk et))).
+    gpu_pts_to_vec' x ((k * nthr + tid) * chunk et)
+      s (i + (k * nthr + tid) * chunk et)
+
+let thread_live_chunks
+  (#et : Type0) {| sized et, has_vec_cpy et |}
+  (#n : nat)
+  ([@@@mkey] x : gpu_array et n)
+  (nthr : nat)
+  (tid : natlt nthr)
+: Pure slprop
+  (requires (nthr * chunk et) /? n)
+  (ensures fun _ -> true)
+=
+  forall+ (k : natlt (n / (nthr * chunk et))).
+    gpu_live_vec x ((k * nthr + tid) * chunk et)
+
+
+
+(* Helpers *)
+
+open Kuiper.Bijection
+
+// TODO por que esto no está definido?
+ghost
+fn gpu_array_slice_1'
+  (#a:Type u#0)
+  (#sz:nat)
+  (arr : gpu_array a sz)
+  (#f : perm)
+  (i j : natle sz)
+  (#v : erased (seq a){ Seq.length v == j - i })
+  requires gpu_pts_to_slice arr #f i j v
+  ensures  forall+ (k: natlt (j - i)). gpu_pts_to_cell arr #f (i + k) (v @! k)
+{
+  admit()
+}
+
+ghost
+fn gpu_array_unslice_1'
+  (#a:Type u#0)
+  (#sz:nat)
+  (arr : gpu_array a sz)
+  (#f : perm)
+  (i j : natle sz)
+  (#v : erased (seq a) { Seq.length v == j - i })
+  requires forall+ (k: natlt (j - i)). gpu_pts_to_cell arr #f (i + k) (v @! k)
+  ensures gpu_pts_to_slice arr #f i j v
+{
+  admit();
+}
+
+let share_thread_ff
+  (n : nat) (nthr : pos) (k : natlt n)
+: (tid : natlt nthr & natlt ((n + (nthr - 1) - tid) / nthr))
+= (| k % nthr, k / nthr |)
+
+let share_thread_gg
+  (n : nat) (nthr : pos)
+  (tid : natlt nthr) (k : natlt ((n - tid) `divup` nthr))
+: (natlt n)
+= (k * nthr + tid)
+
+let share_thread_bij (n : nat) (nthr : pos)
+: bijection
+  (natlt n)
+  (tid : natlt nthr & natlt ((n - tid) `divup` nthr))
+=
+{
+  ff = (fun k -> share_thread_ff n nthr k);
+  gg = (fun (| tid, k |) -> share_thread_gg n nthr tid k);
+
+  ff_gg = ez;
+  gg_ff = ez;
+}
+
+ghost
+fn thread_slice_share
+  (#et : Type0)
+  (#n : nat)
+  (x : gpu_array et n)
+  (i j : natle n { i <= j })
+  (#m : nat)
+  (nthr : pos)
+  requires slice_live x i j
+  ensures forall+ (tid : natlt nthr). thread_slice_live x i j nthr tid
+{
+  unfold slice_live;
+  with s. assert gpu_pts_to_slice x i j s;
+  gpu_pts_to_slice_ref x i j;
+
+  gpu_array_slice_1' x i j;
+  forevery_iso (share_thread_bij (j - i) nthr) _;
+  forevery_ext
+    (fun r -> 
+      gpu_pts_to_cell x
+        (i + (share_thread_bij (j - i) nthr).gg r)
+        (s @! (share_thread_bij (j - i) nthr).gg r)
+    )
+    (fun (| tid, k |) ->
+      gpu_pts_to_cell x (i + k * nthr + tid ) (s @! k * nthr + tid)
+    );
+  forevery_unflatten_dep' _;
+
+  forevery_map #(natlt nthr)
+    (fun tid -> forall+ (k : natlt (((j -i) - tid) `divup` nthr)).
+      gpu_pts_to_cell x (i + k * nthr + tid) (s @! k * nthr + tid)
+    ) 
+    (fun tid -> thread_slice_live x i j nthr tid)
+    fn tid {
+      forevery_map #(natlt (((j -i) - tid) `divup` nthr))
+        (fun k -> gpu_pts_to_cell x (i + k * nthr + tid) (s @! k * nthr + tid))
+        (fun k -> array_live_cell x (i + k * nthr + tid))
+        fn k {
+          fold array_live_cell x (i + k * nthr + tid);
+        };
+      fold thread_slice_live x i j nthr tid;
+    };
+}
+
+ghost
+fn thread_slice_gather
+  (#et : Type0)
+  (#n : nat)
+  (x : gpu_array et n)
+  (i j : natle n { i <= j })
+  (#m : nat)
+  (s : lseq et m)
+  (k : natle (m - (j - i)))
+  (nthr : pos)
+  requires forall+ (tid : natlt nthr). thread_slice_pts_to x i j s k nthr tid
+  ensures gpu_pts_to_slice x i j (Seq.slice s k (k + (j - i)))
+{
+  let s' = Seq.slice s k (k + (j - i));
+
+  forevery_map #(natlt nthr)
+    (fun tid -> thread_slice_pts_to x i j s k nthr tid)
+    (fun tid -> forall+ (h : natlt (((j -i) - tid) `divup` nthr)).
+      gpu_pts_to_cell x (i + h * nthr + tid) (s' @! h * nthr + tid)
+    ) 
+    fn tid {
+      unfold thread_slice_pts_to x i j s k nthr tid;
+      forevery_ext #(natlt (((j -i) - tid) `divup` nthr))
+        (fun h -> gpu_pts_to_cell x (i + h * nthr + tid) (s @! k + h * nthr + tid))
+        (fun h -> gpu_pts_to_cell x (i + h * nthr + tid) (s' @! h * nthr + tid));
+    };
+
+  forevery_flatten_dep _;
+
+  forevery_ext #(tid : natlt nthr & natlt (((j - i) - tid) `divup` nthr))
+    (fun r ->
+      gpu_pts_to_cell x (i + r._2 * nthr + r._1) (s' @! r._2 * nthr + r._1)
+    )
+    (fun r -> 
+      gpu_pts_to_cell x
+        (i + (share_thread_bij (j - i) nthr).gg r)
+        (s' @! (share_thread_bij (j - i) nthr).gg r)
+    );
+
+  forevery_iso_back (share_thread_bij (j - i) nthr)
+    (fun r -> gpu_pts_to_cell x (i + r) (s' @! r));
+
+  gpu_array_unslice_1' x i j;
+}
+
+ghost
+fn thread_slice_gather_value
+  (#et : Type0)
+  (#n : nat)
+  (x : gpu_array et n)
+  (i j : natle n { i <= j })
+  (v : et)
+  (nthr : pos)
+  requires forall+ (tid : natlt nthr). thread_slice_pts_to_value x i j v nthr tid
+  ensures gpu_pts_to_slice x i j (Seq.create (j - i) v)
+{
+  let s = Seq.create (j - i) v;
+  forevery_map #(natlt nthr)
+    (fun tid -> thread_slice_pts_to_value x i j v nthr tid)
+    (fun tid -> forall+ (k : natlt (((j -i) - tid) `divup` nthr)).
+      gpu_pts_to_cell x (i + k * nthr + tid) (s @! k * nthr + tid)
+    ) 
+    fn tid {
+      unfold thread_slice_pts_to_value x i j v nthr tid;
+      forevery_ext #(natlt (((j -i) - tid) `divup` nthr))
+        (fun h -> gpu_pts_to_cell x (i + h * nthr + tid) v)
+        (fun h -> gpu_pts_to_cell x (i + h * nthr + tid) (s @! h * nthr + tid));
+    };
+  forevery_flatten_dep _;
+  forevery_ext #(tid : natlt nthr & natlt (((j - i) - tid) `divup` nthr))
+    (fun r ->
+      gpu_pts_to_cell x (i + r._2 * nthr + r._1) (s @! r._2 * nthr + r._1)
+    )
+    (fun r -> 
+      gpu_pts_to_cell x
+        (i + (share_thread_bij (j - i) nthr).gg r)
+        (s @! (share_thread_bij (j - i) nthr).gg r)
+    );
+  forevery_iso_back (share_thread_bij (j - i) nthr)
+    (fun r -> gpu_pts_to_cell x (i + r) (s @! r));
+
+  gpu_array_unslice_1' x i j;
+}
+
+ghost
+fn thread_share_chunks
+  (#et : Type0) {| sized et, has_vec_cpy et |}
+  (#n : nat)
+  (x : gpu_array et n)
+  (nthr : pos)
+  (#_: squash ((nthr * chunk et) /? n))
+  requires live x
+  ensures forall+ (tid : natlt nthr). thread_live_chunks x nthr tid
+{
+  with s. assert gpu_pts_to_slice x 0 n s;
+  gpu_pts_to_slice_ref x 0 n;
+
+  let ch = chunk et;
+
+  gpu_array_slice_1 x;
+
+  forevery_factor n (n / (nthr * ch)) (nthr * ch) _;
+
+  forevery_map #(natlt (n / (nthr * ch)))
+    (fun k ->
+      forall+ (h : natlt (nthr * ch)).
+        gpu_pts_to_cell x (k * (nthr * ch) + h) (s @! k * (nthr * ch) + h)
+    )
+    (fun k ->
+      forall+ (tid : natlt nthr). gpu_live_vec x ((k * nthr + tid) * chunk et)
+    )
+    fn k {
+      forevery_factor (nthr * ch) nthr ch _;
+      forevery_map #(natlt nthr)
+        (fun tid ->
+          forall+ (i : natlt ch).
+            gpu_pts_to_cell x
+              (k * (nthr * ch) + (tid * ch + i))
+              (s @! k * (nthr * ch) + (tid * ch + i))
+        )
+        (fun tid ->
+          gpu_live_vec x ((k * nthr + tid) * chunk et)
+        )
+        fn tid {
+          let v : lseq et ch = Seq.slice s 
+            ((k * nthr + tid) * ch)
+            ((k * nthr + tid) * ch + ch);
+
+          forevery_ext #(natlt ch)
+            _
+            (fun i -> gpu_pts_to_cell x ((k * nthr + tid) * ch + i) (v @! i));
+          forevery_rw_size ch
+            (((k * nthr + tid) * ch) + ch - ((k * nthr + tid) * ch));
+
+          gpu_array_unslice_1' x
+            ((k * nthr + tid) * ch)
+            ((k * nthr + tid) * ch + ch);
+
+          rewrite each ch as (chunk et);
+          fold gpu_live_vec x ((k * nthr + tid) * chunk et);
+        };
+    };
+  rewrite each ch as (chunk et);
+
+  forevery_commute _;
+
+  forevery_map #(natlt nthr)
+    (fun tid ->
+      forall+ (k: natlt (n / (nthr * (chunk et)))).
+        gpu_live_vec x ((k * nthr + tid) * (chunk et))
+    )
+    (fun tid -> thread_live_chunks x nthr tid)
+    fn tid { fold thread_live_chunks x nthr tid };
+}
+
+ghost
+fn thread_gather_chunks
+  (#et : Type0) {| sized et, has_vec_cpy et |}
+  (#n : nat)
+  (x : gpu_array et n)
+  (#m : nat)
+  (s : lseq et m)
+  (i : natle (m - n))
+  (nthr : pos)
+  (#_: squash ((nthr * chunk et) /? n))
+  requires forall+ (tid : natlt nthr). thread_pts_to_chunks x s i nthr tid
+  ensures x |-> Seq.slice s i (i + n)
+{
+  let ch = v (chunk et);
+  forevery_map
+    (fun tid -> thread_pts_to_chunks x s i nthr tid)
+    (fun tid -> 
+      forall+ (j : natlt ch) (k : natlt (n / (nthr * ch))).
+        gpu_pts_to_cell x (k * (nthr * ch) + (tid * ch + j))
+          (s @! i + (k * (nthr * ch) + (tid * ch + j)))
+    )
+    fn tid {
+      unfold thread_pts_to_chunks x s i nthr tid;
+      forevery_map #(natlt (n / (nthr * (chunk et))))
+        (fun k ->
+          gpu_pts_to_vec' x ((k * nthr + tid) * chunk et)
+            s (i + (k * nthr + tid) * chunk et)
+        )
+        (fun k ->
+          forall+ (j : natlt ch).
+            gpu_pts_to_cell x (k * (nthr * ch) + (tid * ch + j))
+              (s @! i + (k * (nthr * ch) + (tid * ch + j)))
+        )
+        fn k {
+          rewrite each (v (chunk et)) as ch;
+
+          gpu_array_slice_1' x
+            ((k * nthr + tid) * ch)
+            ((k * nthr + tid) * ch + ch);
+
+          forevery_rw_size _ ch;
+
+          forevery_ext #(natlt ch)
+            _
+            (fun j ->
+              gpu_pts_to_cell x (k * (nthr * ch) + (tid * ch + j))
+                (s @! i + (k * (nthr * ch) + (tid * ch + j)))
+            );
+          ();
+        };
+      rewrite each (v (chunk et)) as ch;
+      forevery_commute _;
+    };
+
+  forevery_unfactor (nthr * ch) _ _
+    (fun h ->
+      forall+ (k : natlt (n / (nthr * ch))).
+        gpu_pts_to_cell x
+          (k * (nthr * ch) + h)
+          (s @! i + (k * (nthr * ch) + h))
+    );
+  forevery_commute _;
+  forevery_unfactor n (n / (nthr * ch)) (nthr * ch)
+    (fun k -> gpu_pts_to_cell x k (s @! i + k));
+  forevery_ext _
+    (fun (k : natlt n) ->
+      gpu_pts_to_cell x k (Seq.slice s i (i + n) @! k)
+    );
+  gpu_array_unslice_1 x;
+}
